add client 11

VST-introduction/client1.c
@@ -26,7 +26,7 @@ void *kalloc1(void)
   return (void*)r;
 }
 
-// not added to client 1 yet
+// not added to client 1 yet -- it is in simple-kfree
 void freerange_while_loop(void *pa_start, void *pa_end) {  // admit on pointer
   while ((char*)pa_start + PGSIZE <= (char*)pa_end) { 
       kfree1(pa_start);
@@ -34,11 +34,114 @@ void freerange_while_loop(void *pa_start, void *pa_end) {  // admit on pointer
   }
 }
 
-// should return pa..
+// should return pa
 void *client1(void *pa) {
   kfree1(pa);
   return kalloc1();
 }
+
+
+
+// should return pa1
+void *client2(void *pa1, void *pa2) {
+  kfree1(pa1);
+  kfree1(pa2);
+  kalloc1();
+  return kalloc1();
+}
+
+
+// should return pa2
+void *client3(void *pa1, void *pa2) {
+  kfree1(pa1);
+  kfree1(pa2);
+  return kalloc1();
+}
+
+void *client4(void *pa1, void *pa2) {
+  client1(pa1);
+  return client1(pa2);
+}
+
+void *client5(void *pa1, void *pa2) {
+  kfree1(pa1);
+  kalloc1();
+  kfree1(pa2);
+  return kalloc1();
+}
+
+void *client6(void *pa_start) {
+  int i = 0;
+  while (i < 2) {
+      kfree1(pa_start);
+      pa_start = (char*)pa_start + PGSIZE;
+      i++;
+  }
+  return kalloc1();
+}
+
+void *client7(void *pa_start, int n) {
+  int i = 0;
+  while (i < n) {
+      kfree1(pa_start);
+      pa_start = (char*)pa_start + PGSIZE;
+      i++;
+  }
+  return kalloc1();
+}
+
+void client8(void *pa_start, int n) {
+  int i = 0;
+  while (i < n) {
+      kfree1(pa_start);
+      pa_start = (char*)pa_start + PGSIZE;
+      i++;
+  }
+}
+
+// this is basicly doing the same as client 7
+void* client9(void *pa_start, int n) {
+  client8(pa_start, n);
+  return kalloc1();
+}
+
+// this is allowed..
+void client10(void *pa_start) {
+  kfree1(pa_start);
+  kfree1(pa_start);
+}
+
+
+// working in progress.. simple version of pipealloc without allocating the files..
+
+
+#define PIPESIZE 512
+typedef unsigned int   uint;
+
+struct pipe {
+  char data[PIPESIZE];
+  uint nread;     // number of bytes read
+  uint nwrite;    // number of bytes written
+  int readopen;   // read fd is still open
+  int writeopen;  // write fd is still open
+};
+
+// very simple - just to check if it can be used for a pipe..
+void client_11_pipealloc()
+{
+  struct pipe *pi;
+
+  pi = 0;
+  pi = (struct pipe*)kalloc1();
+  if(pi) {
+    pi->readopen = 1;
+    pi->writeopen = 1;
+    pi->nwrite = 0;
+    pi->nread = 0;
+  }
+}
+
+
 
 
 
